...

TestTheories/Sorting.thy
@@ -31,7 +31,8 @@ fun sorted' :: "nat list \<Rightarrow> bool" where
 fun merge :: "nat list \<Rightarrow> nat list \<Rightarrow> nat list" where
   "merge rs [] = rs"
 | "merge [] ts = ts"
-| "merge (r#rs) (t#ts) = (if r \<le> t then r # merge rs (t#ts) else t # merge (r#rs) ts)"
+| "merge (r#rs) (t#ts) = (if r \<le> t then r # merge rs (t#ts)
+                                       else t # merge (r#rs) ts)"
 
 fun msort :: "nat list => nat list" where
   "msort [] = []"
@@ -39,8 +40,7 @@ fun msort :: "nat list => nat list" where
 | "msort ts = merge (msort (List.take (length ts div 2) ts)) (* size instead? *)
                     (msort (List.drop (length ts div 2) ts))"
 
-lemma sortCons: "r \<le> t \<and> sorted' (t # ts) \<Longrightarrow> sorted' (r # (t # ts))"
-by simp
+(* lemma sortCons: "r \<le> t \<and> sorted' (t # ts) \<Longrightarrow> sorted' (r # (t # ts))" by simp *)
 
 lemma mer1: "sorted' ts \<Longrightarrow> sorted' (merge [] ts)"
 (*by(metis sorted'.cases merge.simps)*) (* replace of cases by inductions *)
@@ -52,8 +52,7 @@ by hipster_induct_schemes
 lemma mer3: "sorted' ts \<Longrightarrow> sorted' (merge ts [t])" (* sorted'.induct! *)
 by hipster_induct_schemes
 
-lemma mer4: "sorted' (t # ts) \<and> \<not> t \<le> r \<Longrightarrow> sorted' (r # (merge (t#ts) []))"
-by simp
+lemma mer4: "sorted' (t # ts) \<and> \<not> t \<le> r \<Longrightarrow> sorted' (r # (merge (t#ts) []))" by simp
 
 lemma mer4': "sorted' (t # ts) \<and> t \<le> r \<Longrightarrow> sorted' (t # merge ts [r])"
 by (hipster_induct_schemes merge.simps mer3)
@@ -67,17 +66,18 @@ by (hipster_induct_schemes merge.simps mer3)
 lemma mer5'': "sorted' (r # rs) \<and> \<not> t \<le> r \<Longrightarrow> sorted' (r # (merge [t] rs))"
 by (hipster_induct_schemes sorted'.simps)
 
-(*lemma merComm: "sorted' ts \<and> sorted' rs \<Longrightarrow> merge rs ts = merge ts rs"
-apply(induction rs ts rule: merge.induct)
-apply(simp_all)
-apply(metis sorted'.cases merge.simps(1) merge.simps(2))*)
+lemma ssu: "sorted' (r # rs) \<and> t \<le> r \<Longrightarrow> sorted' (t # (merge [] (r#rs)))" by (metis merge.simps sorted'.simps)
+(*by (hipster_induct_simp_metis)*)
+
+lemma ssu': "sorted' (r # rs) \<and> t \<le> v \<and> t \<le> r \<Longrightarrow> sorted' (t # (merge [v] (r#rs)))"
+by (metis mer5'' merge.simps sorted'.simps)
 
 (* simplification can very much screw up the goal state! *)
 lemma mer5: "(sorted' (t # ts) \<and> sorted' (r # rs) \<and> t \<le> r) \<Longrightarrow> (sorted' (t # (merge ts (r#rs))))"
 apply(induction ts rule: sorted'.induct)
 apply(simp)
 apply(simp add: mer5'')
-apply(simp add: mer5' mer4') (*
+apply(simp add: ssu ssu' mer5' mer4') (*
 apply(metis merge.simps(3) mer5' mer4' mer3 mer4)*)
 sorry
 
@@ -86,12 +86,13 @@ by hipster_induct_simp_metis
 (*by (metis sorted'.elims(3) sorted'.simps(3))*)
 
 lemma mergeS: "sorted' ts \<and> sorted' rs \<Longrightarrow> sorted' (merge ts rs)"
-(* apply(induction ts rs rule: merge.induct)
+apply(induction ts rs rule: merge.induct)
 apply(simp_all add: mer1 mer2)
-by (metis mer4 mer5 merge.simps sorted'.simps)*)
+by (metis mer4 mer5 merge.simps sorted'.simps)
+(*
 apply(cases rs)
 apply(simp_all)
-by (hipster_induct_schemes mer1 mer5'' mer5 merge.simps sorted'.simps)
+by (hipster_induct_schemes mer1 mer5'' mer5 merge.simps sorted'.simps)*)
 (*apply(induction ts rule: sorted'.induct)
 apply(simp add: mer1)
 apply(simp add: mer5'')
@@ -106,6 +107,11 @@ by (metis mer4 mer5 merge.simps sorted'.simps)*)
 
 lemma smsort: "sorted' (msort xs)"
 by (hipster_induct_schemes mergeS)
+
+(*lemma merComm: "sorted' ts \<and> sorted' rs \<Longrightarrow> merge rs ts = merge ts rs"
+apply(induction rs ts rule: merge.induct)
+apply(simp_all)
+apply(metis sorted'.cases merge.simps(1) merge.simps(2))*)
 
 
 
